Update.

src/metalogic/fol/current/prop.lean
@@ -58,11 +58,19 @@ def formula.is_tauto (P : formula) : Prop :=
   ∀ (val : valuation), P.eval val = bool.tt
 
 
-def map_val (val : valuation) (P : formula) : formula :=
-if val P = bool.tt then P else P.not_
+@[derive inhabited]
+def assignment : Type := formula → bool
 
-def eval_ff_to_not (val : valuation) (P : formula) : formula :=
-if formula.eval val P = bool.tt then P else P.not_
+def formula.assign (f : assignment) : formula → bool
+| (true_) := f true_
+| (pred_ name args) := f (pred_ name args)
+| (eq_ x y) := f (eq_ x y)
+| (not_ P) := ! P.assign
+| (imp_ P Q) := (! P.assign) || Q.assign
+| (forall_ x P) := f (forall_ x P)
+
+def assign_ff_to_not (f : assignment) (P : formula) : formula :=
+if formula.assign f P = bool.tt then P else P.not_
 
 
 theorem T_13_5
@@ -761,11 +769,11 @@ end
 lemma L_15_7
   (P P' : formula)
   (Δ_U : finset formula)
-  (val : valuation)
+  (f : assignment)
   (Δ_U' : finset formula)
   (h1 : P.atomic_set ⊆ Δ_U)
-  (h2 : Δ_U' = Δ_U.image (eval_ff_to_not val))
-  (h3 : P' = eval_ff_to_not val P) :
+  (h2 : Δ_U' = Δ_U.image (assign_ff_to_not f))
+  (h3 : P' = assign_ff_to_not f P) :
   is_deduct Δ_U' P' :=
 begin
   subst h2,
@@ -773,11 +781,18 @@ begin
   induction P,
   case formula.true_
   {
-    unfold eval_ff_to_not,
-    unfold formula.eval,
-    simp only [eq_self_iff_true, if_true],
-    apply is_deduct.axiom_,
-    exact is_axiom.prop_true_,
+    let P := true_,
+
+    unfold formula.atomic_set at h1,
+    simp only [finset.singleton_subset_iff] at h1,
+
+    unfold assign_ff_to_not,
+    unfold formula.assign,
+
+    apply is_deduct.assume_,
+    simp only [finset.coe_image, set.mem_image, finset.mem_coe],
+    apply exists.intro P,
+    tauto,
   },
   case formula.pred_ : name args
   {
@@ -786,8 +801,8 @@ begin
     unfold formula.atomic_set at h1,
     simp only [finset.singleton_subset_iff] at h1,
 
-    unfold eval_ff_to_not,
-    unfold formula.eval,
+    unfold assign_ff_to_not,
+    unfold formula.assign,
 
     apply is_deduct.assume_,
     simp only [finset.coe_image, set.mem_image, finset.mem_coe],
@@ -801,8 +816,8 @@ begin
     unfold formula.atomic_set at h1,
     simp only [finset.singleton_subset_iff] at h1,
 
-    unfold eval_ff_to_not,
-    unfold formula.eval,
+    unfold assign_ff_to_not,
+    unfold formula.assign,
 
     apply is_deduct.assume_,
     simp only [finset.coe_image, set.mem_image, finset.mem_coe],
@@ -813,10 +828,10 @@ begin
   {
     unfold formula.atomic_set at h1,
 
-    unfold eval_ff_to_not at P_ih,
+    unfold assign_ff_to_not at P_ih,
 
-    unfold eval_ff_to_not,
-    unfold formula.eval,
+    unfold assign_ff_to_not,
+    unfold formula.assign,
 
     simp only [bnot_eq_tt_iff_not_eq_tt],
     split_ifs,
@@ -842,11 +857,11 @@ begin
     simp only [finset.union_subset_iff] at h1,
     cases h1,
 
-    unfold eval_ff_to_not at P_ih,
-    unfold eval_ff_to_not at Q_ih,
+    unfold assign_ff_to_not at P_ih,
+    unfold assign_ff_to_not at Q_ih,
 
-    unfold eval_ff_to_not,
-    unfold formula.eval,
+    unfold assign_ff_to_not,
+    unfold formula.assign,
     simp only [bor_eq_true_eq_eq_tt_or_eq_tt],
     simp only [bnot_eq_tt_iff_not_eq_tt],
     split_ifs,
@@ -905,8 +920,8 @@ begin
     unfold formula.atomic_set at h1,
     simp only [finset.singleton_subset_iff] at h1,
 
-    unfold eval_ff_to_not,
-    unfold formula.eval,
+    unfold assign_ff_to_not,
+    unfold formula.assign,
 
     apply is_deduct.assume_,
     simp only [finset.coe_image, set.mem_image, finset.mem_coe],
@@ -944,26 +959,19 @@ end
 
 lemma lem_2
   (P P' : formula)
-  (val : valuation)
+  (f : assignment)
   (h1 : P.is_atomic) :
-  eval_ff_to_not (function.update_ite val P' tt) P =
-    function.update_ite (eval_ff_to_not val) P' P P :=
+  assign_ff_to_not (function.update_ite f P' tt) P =
+    function.update_ite (assign_ff_to_not f) P' P P :=
 begin
   induction P,
-  case formula.true_
-  {
-    unfold function.update_ite,
-    unfold eval_ff_to_not,
-    unfold formula.eval,
-    simp only [eq_self_iff_true, if_true, if_t_t],
-  },
-  case [formula.pred_, formula.eq_, formula.forall_]
+  case [formula.true_, formula.pred_, formula.eq_, formula.forall_]
   {
     all_goals
     {
       unfold function.update_ite,
-      unfold eval_ff_to_not,
-      unfold formula.eval,
+      unfold assign_ff_to_not,
+      unfold formula.assign,
       unfold function.update_ite,
       split_ifs,
       all_goals {tauto},
@@ -980,15 +988,61 @@ begin
 end
 
 
-example
+lemma lem_3
+  (P P' : formula)
+  (f : assignment)
+  (h1 : P.is_atomic) :
+  assign_ff_to_not (function.update_ite f P' ff) P =
+    function.update_ite (assign_ff_to_not f) P' P.not_ P :=
+begin
+  induction P,
+  case [formula.true_, formula.pred_, formula.eq_, formula.forall_]
+  {
+    all_goals
+    {
+      unfold function.update_ite,
+      unfold assign_ff_to_not,
+      unfold formula.assign,
+      unfold function.update_ite,
+      split_ifs,
+      all_goals {tauto},
+    },
+  },
+  case [formula.not_, formula.imp_]
+  {
+    all_goals
+    {
+      unfold formula.is_atomic at h1,
+      contradiction,
+    }
+  },
+end
+
+
+lemma lem_4
   (P U : formula)
-  (h1 : ∀ (val : valuation), is_deduct {eval_ff_to_not val U} P)
+  (h1 : ∀ (f : assignment), is_deduct {assign_ff_to_not f U} P)
   (h2 : U.is_atomic) :
-  ∀ (val : valuation), is_deduct {U} P :=
+  ∀ (f : assignment), is_deduct {U} P :=
 begin
   intros val,
   specialize h1 (function.update_ite val U bool.tt),
   simp only [lem_2 U U val h2] at h1,
+  unfold function.update_ite at h1,
+  simp only [eq_self_iff_true, if_true] at h1,
+  exact h1,
+end
+
+
+lemma lem_5
+  (P U : formula)
+  (h1 : ∀ (f : assignment), is_deduct {assign_ff_to_not f U} P)
+  (h2 : U.is_atomic) :
+  ∀ (f : assignment), is_deduct {U.not_} P :=
+begin
+  intros val,
+  specialize h1 (function.update_ite val U bool.ff),
+  simp only [lem_3 U U val h2] at h1,
   unfold function.update_ite at h1,
   simp only [eq_self_iff_true, if_true] at h1,
   exact h1,
@@ -1001,8 +1055,8 @@ example
   (h1_Δ : ∀ (U' : formula), U' ∈ Δ → U'.is_atomic)
   (h1_U : U.is_atomic)
   (h2 : U ∉ Δ)
-  (h3 : ∀ (val : valuation), is_deduct ((eval_ff_to_not val U) :: (Δ.map (eval_ff_to_not val))).to_finset P) :
-  ∀ (val : valuation), is_deduct (U :: (Δ.map (eval_ff_to_not val))).to_finset P :=
+  (h3 : ∀ (f : assignment), is_deduct ((assign_ff_to_not f U) :: (Δ.map (assign_ff_to_not f))).to_finset P) :
+  ∀ (f : assignment), is_deduct (U :: (Δ.map (assign_ff_to_not f))).to_finset P :=
 begin
   intros val,
   specialize h3 (function.update_ite val U bool.tt),
@@ -1010,7 +1064,7 @@ begin
   unfold function.update_ite at h3,
   simp only [eq_self_iff_true, if_true] at h3,
 
-  have s1 : list.map (eval_ff_to_not (function.update_ite val U tt)) Δ = list.map (eval_ff_to_not val) Δ,
+  have s1 : list.map (assign_ff_to_not (function.update_ite val U tt)) Δ = list.map (assign_ff_to_not val) Δ,
   {
     simp only [list.map_eq_map_iff],
     intros U' a1,
@@ -1028,18 +1082,46 @@ begin
 end
 
 
-def finset.decreasing_induction
-  {α : Type}
-  [decidable_eq α]
-  (P : finset α → Prop)
-  (U V : finset α)
-  (h1 : ∀ (S : finset α) (x : α), P S → P (S \ {x}))
-  (h2 : U ⊆ V)
-  (h3 : P V) :
-  P U :=
+example
+  (P U : formula)
+  (Δ : list formula)
+  (h1_Δ : ∀ (U' : formula), U' ∈ Δ → U'.is_atomic)
+  (h1_U : U.is_atomic)
+  (h2 : U ∉ Δ)
+  (h3 : ∀ (f : assignment), is_deduct ((assign_ff_to_not f U) :: (Δ.map (assign_ff_to_not f))).to_finset P) :
+  ∀ (f : assignment), is_deduct (U.not_ :: (Δ.map (assign_ff_to_not f))).to_finset P :=
 begin
-  sorry,
+  intros val,
+  specialize h3 (function.update_ite val U bool.ff),
+  simp only [lem_3 U U val h1_U] at h3,
+  unfold function.update_ite at h3,
+  simp only [eq_self_iff_true, if_true] at h3,
+
+  have s1 : list.map (assign_ff_to_not (function.update_ite val U ff)) Δ = list.map (assign_ff_to_not val) Δ,
+  {
+    simp only [list.map_eq_map_iff],
+    intros U' a1,
+    specialize h1_Δ U' a1,
+    simp only [lem_3 U' U val h1_Δ],
+    unfold function.update_ite,
+    simp only [ite_eq_right_iff],
+    intros a2,
+    subst a2,
+    contradiction,
+  },
+
+  rewrite <- s1,
+  exact h3,
 end
+
+
+lemma finset.decreasing_induction_on
+  (S : finset formula)
+  (P : finset formula → Prop)
+  (h1 : P S)
+  (h2 : ∀ (S' : finset formula) (U : formula),
+    S' ⊆ S → P S' → U ∈ S' → P (S' \ {U})) :
+  ∀ (S' : finset formula), S' ⊆ S → P S' := sorry
 
 
 theorem prop_complete
@@ -1047,29 +1129,9 @@ theorem prop_complete
   (h1 : P.is_tauto) :
   is_proof P :=
 begin
+  unfold formula.is_tauto at h1,
+
   unfold is_proof,
-
-  let Δ_U := P.atomic_set,
-  let Δ_U' := fun (val : valuation), Δ_U.image (eval_ff_to_not val),
-  let P' := fun (val : valuation), eval_ff_to_not val P,
-
-  have s1 : ∀ (val : valuation), is_deduct (Δ_U' val) (P' val),
-  sorry,
-
-  have s2 : ∀ (val : valuation), is_deduct (Δ_U' val) P,
-  sorry,
-
-  have s3 : ∀ (val : valuation) (U : formula),
-    U ∈ Δ_U → is_deduct (Δ_U' val \ {eval_ff_to_not val U} ∪ {U}) P,
-  sorry,
-
-  have s4 : ∀ (val : valuation) (U : formula),
-    U ∈ Δ_U → is_deduct (Δ_U' val \ {eval_ff_to_not val U} ∪ {U.not_}) P,
-  sorry,
-
-  have s5 : ∀ (val : valuation) (U : formula),
-    U ∈ Δ_U → is_deduct (Δ_U' val \ {eval_ff_to_not val U}) P,
-  sorry,
 
   sorry,
 end
